Update timing proofs and start a few more

timing/examples/FreeRTOS/strlen.v
@@ -11,47 +11,46 @@ Definition time_mem : N :=
 Definition time_branch : N :=
     5 + (ML - 1).
 
-Module vTaskSuspendAllTime <: TimingModule.
+Module strlenTime <: TimingModule.
     Definition time_of_addr (s : store) (a : addr) : N :=
         match neorv32_cycles_upper_bound ML s (RTOSDemo_NoAsserts_Clz a) with
         | Some x => x | _ => 999 end.
 
-    Definition entry_addr : N := 0x80000d14.
+    Definition entry_addr : N := 0x8000fe7c.
 
     Definition exits (t:trace) : bool :=
     match t with (Addr a,_)::_ => match a with
-    | 0x80000d20 => true
+    | 0x8000fed4 | 0x8000fef4 | 0x8000fefc | 0x8000ff04 => true
     | _ => false
   end | _ => false end.
-End vTaskSuspendAllTime.
+End strlenTime.
+Module strlenAuto := TimingAutomation strlenTime.
+Import strlenTime strlenAuto.
 
-Module vTaskSuspendAllAuto := TimingAutomation vTaskSuspendAllTime.
-Import vTaskSuspendAllTime vTaskSuspendAllAuto.
-
-Definition time_of_vTaskSuspendAll (t : trace) :=
+Definition time_of_strlen (t : trace) :=
     cycle_count_of_trace t = 2 + time_branch + 2 * time_mem.
 
-Definition vTaskSuspendAll_timing_invs
+Definition strlen_timing_invs
     (t:trace) : option Prop :=
 match t with (Addr a, s) :: t' => match a with
 | 0x80000d14 => Some (cycle_count_of_trace t' = 0)
-| 0x80000d20 => Some (time_of_vTaskSuspendAll t)
+| 0x80000d20 => Some (time_of_strlen t)
 | _ => None end | _ => None end.
 
-Definition lifted_vTaskSuspendAll : program :=
+Definition lifted_strlen : program :=
     lift_riscv RTOSDemo_NoAsserts_Clz.
 
 (* We use simpl in a few convenient places: make sure it doesn't go haywire *)
 Arguments N.add _ _ : simpl nomatch.
 Arguments N.mul _ _ : simpl nomatch.
 
-Theorem vTaskSuspendAll_timing:
+Theorem strlen_timing:
   forall s t s' x'
          (ENTRY: startof t (x',s') = (Addr entry_addr, s))
          (MDL: models rvtypctx s),
   satisfies_all 
-    lifted_vTaskSuspendAll
-    (vTaskSuspendAll_timing_invs)
+    lifted_strlen
+    (strlen_timing_invs)
     exits
   ((x',s')::t).
 Proof using.
@@ -69,7 +68,7 @@ Proof using.
 
     destruct_inv 32 PRE.
 
-    repeat step. unfold time_of_vTaskSuspendAll.
-    hammer. rewrite PRE. unfold time_branch, time_mem. psimpl. lia.
+    repeat step. unfold time_of_strlen.
+    hammer. find_rewrites. unfold time_branch, time_mem. lia.
 Qed.
 
