timing/examples/FreeRTOS/tasks/prvResetNextTaskUnblockTime.v
@@ -1,0 +1,88 @@
+Require Import RTOSDemo_NoAsserts_Clz.
+Require Import riscvTiming.
+Import RISCVNotations.
+Require Import timing_auto.
+
+Variable ML : N.
+Variable ML_pos : 1 <= ML.
+
+Definition time_mem : N :=
+    5 + (ML - 2).
+Definition time_branch : N :=
+    5 + (ML - 1).
+
+Module prvResetNextTaskUnblockTimeTime <: TimingModule.
+    Definition time_of_addr (s : store) (a : addr) : N :=
+        match neorv32_cycles_upper_bound ML s (RTOSDemo_NoAsserts_Clz a) with
+        | Some x => x | _ => 999 end.
+
+    Definition entry_addr : N := 0x80000478.
+
+    Definition exits (t:trace) : bool :=
+    match t with (Addr a,_)::_ => match a with
+    | 0x8000048c => true
+    | _ => false
+  end | _ => false end.
+End prvResetNextTaskUnblockTimeTime.
+
+Module prvResetNextTaskUnblockTimeAuto := TimingAutomation prvResetNextTaskUnblockTimeTime.
+Import prvResetNextTaskUnblockTimeTime prvResetNextTaskUnblockTimeAuto.
+
+Definition time_of_prvResetNextTaskUnblockTime (mem : addr -> N) (gp : N) (t : trace) :=
+    cycle_count_of_trace t = 2 * time_mem +
+        (if mem Ⓓ[mem Ⓓ[(0 ⊖ 1900) + gp]] =? 0 then 
+            3 + 2
+         else
+            time_branch + 3 * time_mem + time_branch) +
+        time_mem + time_branch.
+
+Definition prvResetNextTaskUnblockTime_timing_invs (s : store) (base_mem : addr -> N) (gp : N)
+    (t:trace) : option Prop :=
+match t with (Addr a, s) :: t' => match a with
+| 0x80000478 => Some (s V_MEM32 = Ⓜbase_mem /\ s R_GP = Ⓓgp /\ cycle_count_of_trace t' = 0)
+| 0x8000048c => Some (time_of_prvResetNextTaskUnblockTime base_mem gp t)
+| _ => None end | _ => None end.
+
+Definition lifted_prvResetNextTaskUnblockTime : program :=
+    lift_riscv RTOSDemo_NoAsserts_Clz.
+
+(* We use simpl in a few convenient places: make sure it doesn't go haywire *)
+Arguments N.add _ _ : simpl nomatch.
+Arguments N.mul _ _ : simpl nomatch.
+
+Theorem prvResetNextTaskUnblockTime_timing:
+  forall s t s' x' base_mem gp
+         (ENTRY: startof t (x',s') = (Addr entry_addr, s))
+         (MDL: models rvtypctx s)
+         (MEM: s V_MEM32 = Ⓜbase_mem)
+         (GP: s R_GP = Ⓓgp),
+  satisfies_all 
+    lifted_prvResetNextTaskUnblockTime
+    (prvResetNextTaskUnblockTime_timing_invs s base_mem gp)
+    exits
+  ((x',s')::t).
+Proof using.
+    intros.
+    apply prove_invs.
+    Local Ltac step := time rv_step.
+
+    simpl. rewrite ENTRY. unfold entry_addr. step. auto.
+    
+    intros.
+    eapply startof_prefix in ENTRY; try eassumption.
+    eapply preservation_exec_prog in MDL; 
+        try eassumption; [idtac|apply lift_riscv_welltyped].
+    clear - ENTRY PRE MDL. rename t1 into t. rename s1 into s'.
+
+    destruct_inv 32 PRE.
+
+    destruct PRE as (MEM & GP & Cycles).
+    repeat step.
+    unfold time_of_prvResetNextTaskUnblockTime.
+        hammer. find_rewrites.
+        unfold time_mem, time_branch. lia.
+    unfold time_of_prvResetNextTaskUnblockTime.
+        hammer. find_rewrites.
+        unfold time_mem, time_branch. lia. 
+Qed.
+
