timing/examples/FreeRTOS/tasks/prvSearchForNameWithinSingleList.v
@@ -1,0 +1,136 @@
+(* Problem with this function - it contains what is essentially a strcmp, I don't
+   want to deal with the break in the middle of it right now *)
+
+Require Import RTOSDemo_NoAsserts_Clz.
+Require Import riscvTiming.
+Import RISCVNotations.
+Require Import timing_auto.
+
+Variable ML : N.
+Variable ML_pos : 1 <= ML.
+
+Definition time_mem : N :=
+    5 + (ML - 2).
+Definition time_branch : N :=
+    5 + (ML - 1).
+
+Module prvSearchForNameWithinSingleListTime <: TimingModule.
+    Definition time_of_addr (s : store) (a : addr) : N :=
+        match neorv32_cycles_upper_bound ML s (RTOSDemo_NoAsserts_Clz a) with
+        | Some x => x | _ => 999 end.
+
+    Definition entry_addr : N := 0x80000114.
+
+    Definition exits (t:trace) : bool :=
+    match t with (Addr a,_)::_ => match a with
+    | 0x80000130 | 0x80000168 => true
+    | _ => false
+  end | _ => false end.
+End prvSearchForNameWithinSingleListTime.
+
+Module prvSearchForNameWithinSingleListAuto := TimingAutomation prvSearchForNameWithinSingleListTime.
+Import prvSearchForNameWithinSingleListTime prvSearchForNameWithinSingleListAuto.
+
+Definition pvOwner (mem : addr -> N) (a : addr) : addr :=
+    mem Ⓓ[12 + a].
+Definition pxNext (mem : addr -> N) (a : addr) : addr :=
+    mem Ⓓ[8 + a].
+(* https://github.com/FreeRTOS/FreeRTOS-Kernel/blob/main/include/list.h#L172 *)
+Definition uxNumberOfItems (mem : addr -> N) (a : addr) : N :=
+    mem Ⓓ[a].
+Definition xListEnd (mem : addr -> N) (a : addr) : addr :=
+    mem Ⓓ[8 + a].
+(* I think this is due to the compiler flattening the List_t and MiniListItem_t structs *)
+Definition listGET_HEAD_ENTRY (mem : addr -> N) (a : addr) : addr :=
+    mem Ⓓ[12 + a].
+Definition pcTaskName (mem : addr -> N) (a : addr) : addr :=
+    mem Ⓑ[52 + a].
+
+Fixpoint linked_list_length (mem : addr -> N) (list item : addr) (max : nat) : N :=
+    match max with
+    | O => 0
+    | S max' => 
+        if item =? xListEnd mem list then
+            0
+        else
+            1 + linked_list_length mem list (pxNext mem item) max'
+    end.
+
+Definition time_of_prvSearchForNameWithinSingleList (t : trace) 
+      (mem : addr -> N) (pxList pcNameToQuery : addr) (match_idx : option N) :=
+  cycle_count_of_trace t = time_mem +
+    (if negb (uxNumberOfItems mem pxList =? 0) then (
+      3 + time_mem + 2 + 2 +
+      (match match_idx with 
+      | None => linked_list_length mem pxList (listGET_HEAD_ENTRY mem pxList) (Nat.pow 2 32)
+      | Some idx => idx
+      end) (* number of loop iterations *) *
+      (if listGET_HEAD_ENTRY mem pxList =? 8 ⊕ pxList (* &(pxList->xListEnd) *) then
+         3 + 2 + time_branch
+       else (
+         time_mem + 2 + 2 + time_mem + 2 + time_mem + 3)
+      ) (* loop body duration *)
+    )
+    else (
+      time_branch + 2 + time_branch
+    )).
+
+Definition prvSearchForNameWithinSingleList_timing_invs 
+    (base_mem : addr -> N) (a0 a1 : N) (t:trace) : option Prop :=
+match t with (Addr a, s) :: t' => match a with
+| 0x80000114 => Some (s V_MEM32 = Ⓜbase_mem /\ s R_A0 = Ⓓa0 /\ s R_A1 = Ⓓa1 /\
+                        cycle_count_of_trace t' = 0)
+| 0x80000130 | 0x80000168 => Some (time_of_prvSearchForNameWithinSingleList t base_mem a0)
+| _ => None end | _ => None end.
+
+Definition lifted_prvSearchForNameWithinSingleList : program :=
+    lift_riscv RTOSDemo_NoAsserts_Clz.
+
+(* We use simpl in a few convenient places: make sure it doesn't go haywire *)
+Arguments N.add _ _ : simpl nomatch.
+Arguments N.mul _ _ : simpl nomatch.
+
+Theorem prvSearchForNameWithinSingleList_timing:
+  forall s t s' x' base_mem a0 a1
+         (ENTRY: startof t (x',s') = (Addr entry_addr, s))
+         (MDL: models rvtypctx s)
+         (MEM: s V_MEM32 = Ⓜbase_mem)
+         (A0: s R_A0 = Ⓓa0)
+         (A1: s R_A1 = Ⓓa1),
+  satisfies_all 
+    lifted_prvSearchForNameWithinSingleList
+    (prvSearchForNameWithinSingleList_timing_invs base_mem a0 a1)
+    exits
+  ((x',s')::t).
+Proof using.
+    intros.
+    apply prove_invs.
+    Local Ltac step := time rv_step.
+
+    simpl. rewrite ENTRY. unfold entry_addr. step. auto.
+
+    intros.
+    eapply startof_prefix in ENTRY; try eassumption.
+    eapply preservation_exec_prog in MDL; 
+        try eassumption; [idtac|apply lift_riscv_welltyped].
+    clear - ENTRY PRE MDL. rename t1 into t. rename s1 into s'.
+
+    destruct_inv 32 PRE.
+
+    destruct PRE as (MEM & A0 & Cycles).
+    step. step. (* 0x80000118: beqz a5,8000012c *)
+    - (* m[a0] = 0, postcondition *)
+      repeat step. unfold time_of_prvSearchForNameWithinSingleList, uxNumberOfItems, listGET_HEAD_ENTRY.
+      hammer. find_rewrites. unfold time_mem, time_branch. lia.
+    - (* m[a0] != 0 *)
+      step. step. step. step. (* 0x80000128: bne a4,a2,80000134 *)
+      -- (* m [12 + a0] != 8 + n *)
+          step. step. step. step. step. step. step.
+      -- (* m [12 + a0] = 8 + n *)
+          step. (* postcondition *)
+          unfold time_of_prvSearchForNameWithinSingleList, uxNumberOfItems, listGET_HEAD_ENTRY.
+          hammer. change ((8 + a0) mod 4294967296) with (8 ⊕ a0). find_rewrites.
+          psimpl. cbn [negb]. unfold time_mem, time_branch. apply Bool.negb_false_iff in BC0.
+          rewrite BC0. lia.
+Qed.
+
