timing/examples/FreeRTOS/tasks/vTaskSuspendAll.v
@@ -1,0 +1,75 @@
+Require Import RTOSDemo_NoAsserts_Clz.
+Require Import riscvTiming.
+Import RISCVNotations.
+Require Import timing_auto.
+
+Variable ML : N.
+Variable ML_pos : 1 <= ML.
+
+Definition time_mem : N :=
+    5 + (ML - 2).
+Definition time_branch : N :=
+    5 + (ML - 1).
+
+Module vTaskSuspendAllTime <: TimingModule.
+    Definition time_of_addr (s : store) (a : addr) : N :=
+        match neorv32_cycles_upper_bound ML s (RTOSDemo_NoAsserts_Clz a) with
+        | Some x => x | _ => 999 end.
+
+    Definition entry_addr : N := 0x80000d14.
+
+    Definition exits (t:trace) : bool :=
+    match t with (Addr a,_)::_ => match a with
+    | 0x80000d20 => true
+    | _ => false
+  end | _ => false end.
+End vTaskSuspendAllTime.
+
+Module vTaskSuspendAllAuto := TimingAutomation vTaskSuspendAllTime.
+Import vTaskSuspendAllTime vTaskSuspendAllAuto.
+
+Definition time_of_vTaskSuspendAll (t : trace) :=
+    cycle_count_of_trace t = 2 + time_branch + 2 * time_mem.
+
+Definition vTaskSuspendAll_timing_invs
+    (t:trace) : option Prop :=
+match t with (Addr a, s) :: t' => match a with
+| 0x80000d14 => Some (cycle_count_of_trace t' = 0)
+| 0x80000d20 => Some (time_of_vTaskSuspendAll t)
+| _ => None end | _ => None end.
+
+Definition lifted_vTaskSuspendAll : program :=
+    lift_riscv RTOSDemo_NoAsserts_Clz.
+
+(* We use simpl in a few convenient places: make sure it doesn't go haywire *)
+Arguments N.add _ _ : simpl nomatch.
+Arguments N.mul _ _ : simpl nomatch.
+
+Theorem vTaskSuspendAll_timing:
+  forall s t s' x'
+         (ENTRY: startof t (x',s') = (Addr entry_addr, s))
+         (MDL: models rvtypctx s),
+  satisfies_all 
+    lifted_vTaskSuspendAll
+    (vTaskSuspendAll_timing_invs)
+    exits
+  ((x',s')::t).
+Proof using.
+    intros.
+    apply prove_invs.
+    Local Ltac step := time rv_step.
+
+    simpl. rewrite ENTRY. unfold entry_addr. step. reflexivity.
+    
+    intros.
+    eapply startof_prefix in ENTRY; try eassumption.
+    eapply preservation_exec_prog in MDL; 
+        try eassumption; [idtac|apply lift_riscv_welltyped].
+    clear - ENTRY PRE MDL. rename t1 into t. rename s1 into s'.
+
+    destruct_inv 32 PRE.
+
+    repeat step. unfold time_of_vTaskSuspendAll.
+    hammer. find_rewrites. unfold time_branch, time_mem. lia.
+Qed.
+
